add progress and preservation for records

tapl/tapl/s15subtyping.lean
@@ -6,26 +6,24 @@ namespace Subtyping
 
 abbrev Label := String
 
-mutual
+#check List.Nodup
+
+structure SList (α : Type*) [DecidableEq α] [Inhabited α] where
+  elems : List α
+  nodup : elems.Nodup
+
+
+instance (α : Type*) [DecidableEq α] [Inhabited α] : Inhabited (SList α) where
+  default := ⟨[], by simp⟩
+
 inductive type
 | boolean
 | nat
 | arr (tp : type) (ct : type)
-| rcd (tp: rcd_type)
+| rcd (tps : List type) (tpl : SList Label)
 | top
+deriving Inhabited
 
-inductive rcd_type
-| rcd_nil
-| rcd_cons (l : Label) (hd : type) (tl : rcd_type)
-end
-
-def rcd_type.proj (rcd : rcd_type) (l : Label) : Option type :=
-match rcd with
-| rcd_type.rcd_nil => none
-| rcd_type.rcd_cons l' hd tl =>
-  if l = l' then some hd else rcd_type.proj tl l
-
-mutual
 inductive Term
 | trueT : Term
 | falseT : Term
@@ -37,44 +35,36 @@ inductive Term
 | Succ (t : Term)
 | Pred (t : Term)
 | IsZero (t : Term)
-| Rcd (t : RcdTerm)
+| Rcd (tpt : List Term) (tpl : SList Label)
 | Proj (t : Term) (l : Label)
-
-inductive RcdTerm
-| RcdNil
-| RcdCons (l : Label) (hd : Term) (tl : RcdTerm)
-end
+deriving Inhabited
 
 inductive NatValue : Term → Prop
 | ZeroV : NatValue .Zero
 | SuccV (t : Term) : NatValue t → NatValue (.Succ t)
-
-mutual
-inductive RcdValue : RcdTerm → Prop
-| RcdNilV : RcdValue RcdTerm.RcdNil
-| RcdConsV (l : Label) (hd : Term) (tl : RcdTerm) :
-  Value hd → RcdValue tl → RcdValue (RcdTerm.RcdCons l hd tl)
 
 inductive Value : Term → Prop
 | Abs (t : Term) (tp : type) : Value (t.Abs tp)
 | trueV : Value .trueT
 | falseV : Value .falseT
 | NatV (t : Term) : NatValue t → Value t
-| RcdV (t : RcdTerm) : RcdValue t → Value (Term.Rcd t)
-end
+| RcdV (tpt : List Term) (tpl : SList Label) :
+  (∀ i < tpt.length, Value tpt[i]!) →
+  Value (Term.Rcd tpt tpl)
 
 abbrev TCtx := List type
 
 @[simp, grind]
 def TCtx.types (Γ : TCtx) (x : Nat) (tp : type) : Prop := Γ[x]? = tp
 
-mutual
-inductive RcdTyp : TCtx → RcdTerm → rcd_type → Prop
-| RcdNil : RcdTyp Γ RcdTerm.RcdNil rcd_type.rcd_nil
-| RcdCons (l : Label) (hd : Term) (tl : RcdTerm) (Γ : TCtx)
-          (tp_hd : type) (tp_tl : rcd_type) :
-  Typ Γ hd tp_hd → RcdTyp Γ tl tp_tl →
-  RcdTyp Γ (RcdTerm.RcdCons l hd tl) (rcd_type.rcd_cons l tp_hd tp_tl)
+-- For keys specifically
+theorem SList.Perm.key_correspondence [DecidableEq α] [Inhabited α]
+    (s t : SList α) (h : s.elems.Perm t.elems)
+    (i : Fin s.elems.length) :
+    ∃ j : Fin t.elems.length,
+      s.elems[i]! = t.elems[j]! := by
+  obtain ⟨j, hj, heq⟩ := List.mem_iff_getElem.mp (h.mem_iff.mp (List.getElem_mem i.isLt))
+  exact ⟨⟨j, hj⟩, by grind⟩
 
 inductive Typ : TCtx → Term → type → Prop
 | Ttrue : Typ Γ .trueT type.boolean
@@ -104,13 +94,23 @@ inductive Typ : TCtx → Term → type → Prop
 | TIsZero (t : Term) (Γ : TCtx) :
   Typ Γ t type.nat →
   Typ Γ (.IsZero t) type.boolean
-| TRcd (t : RcdTerm) (Γ : TCtx) (tp : rcd_type) :
-  RcdTyp Γ t tp → Typ Γ (.Rcd t) (type.rcd tp)
-| TProj (t : Term) (l : Label) (Γ : TCtx) (tp : type) (rcd_tp : rcd_type) :
-  Typ Γ t (type.rcd rcd_tp) →
-  rcd_type.proj rcd_tp l = some tp →
+| TRcd (tpt : List Term) (Γ : TCtx) (tpl₁ tpl₂ : SList Label) (tps : List type) :
+  -- is there a way to do this better?
+  tpt.length = tpl₁.elems.length →
+  tpl₁.elems.Perm tpl₂.elems →
+  tps.length = tpl₂.elems.length →
+  (∀ i j, i < tpl₁.elems.length → j < tpl₂.elems.length → tpl₁.elems[i]! = tpl₂.elems[j]! →
+    Typ Γ tpt[i]! tps[j]!) →
+  Typ Γ (.Rcd tpt tpl₁) (.rcd tps tpl₂)
+| TProj (t : Term) (l : Label) (Γ : TCtx)
+  (tpl : SList Label) (tps : List type) (i : Nat) (tp : type) :
+  -- we can do a step under index even if we have duplicates?
+  Typ Γ t (.rcd tps tpl) →
+  l = tpl.elems[i]! →
+  tp = tps[i]! →
+  i < tps.length →
   Typ Γ (.Proj t l) tp
-end
+
 
 def shift_up_from (c : Nat) : Term → Term
 | .Zero => .Zero
@@ -123,51 +123,31 @@ def shift_up_from (c : Nat) : Term → Term
 | .Abs t tp => .Abs (shift_up_from (c + 1) t) tp
 | .App t1 t2 => .App (shift_up_from c t1) (shift_up_from c t2)
 | .ite ct t1 t2 => .ite (shift_up_from c ct) (shift_up_from c t1) (shift_up_from c t2)
-| .Rcd t => .Rcd (shift_up_from_rcd c t)
+| .Rcd tpt tpl => .Rcd (tpt.map (fun t => shift_up_from c t)) tpl
 | .Proj t l => .Proj (shift_up_from c t) l
-where
-  shift_up_from_rcd (c : Nat) : RcdTerm → RcdTerm
-  | RcdTerm.RcdNil => RcdTerm.RcdNil
-  | RcdTerm.RcdCons l hd tl =>
-    RcdTerm.RcdCons l (shift_up_from c hd) (shift_up_from_rcd c tl)
 
 def shift_up (s : Term) : Term := shift_up_from 0 s
 
-mutual
+/-
+Now this one is simply incorrect:
+formally speaking, {"x" : nat, "y" : bool} and {"y" : bool, "x" : nat}
+are two different types.
+
 lemma TypDet (t : Term) (tp₁ tp₂ : type) (Γ : TCtx) :
   Typ Γ t tp₁ → Typ Γ t tp₂ → tp₁ = tp₂ := by
     intro h1 h2
-    cases t
-    all_goals (
-    try grind [Typ]
-    try {
-      cases h1
-      cases h2
-      have _ := TypDet (by assumption)
-      grind
-    })
-    · rename_i t1 t2
-      cases h1
-      cases h2
-      have _ := TypDet t2
-      have _ := TypDet t1
-      grind
-    · rename_i t
-      cases h1
-      cases h2
-      have _ := RcdTypDet t
-      grind
-
-lemma RcdTypDet (t : RcdTerm) (tp₁ tp₂ : rcd_type) (Γ : TCtx) :
-  RcdTyp Γ t tp₁ → RcdTyp Γ t tp₂ → tp₁ = tp₂ := by
-    intro h1 h2
-    cases t <;> cases h1 <;> cases h2
-    · rfl
-    · rename_i th1 _ _ _ th2 _
-      have _ := TypDet _ _ _ _ th1 th2
-      have _ := RcdTypDet (by assumption)
-      grind
-end
+    unhygienic induction h1 generalizing tp₂
+    all_goals try
+    { cases h2
+      grind }
+    { unhygienic cases h2
+      simp
+      sorry }
+    unhygienic cases h2
+    have lm := a_ih _ a_3
+    simp at lm
+    sorry
+-/
 
 def betar (k : Nat) (t s : Term) : Term :=
   match t with
@@ -181,24 +161,11 @@ def betar (k : Nat) (t s : Term) : Term :=
   | .Succ t => .Succ (betar k t s)
   | .Pred t => .Pred (betar k t s)
   | .IsZero t => .IsZero (betar k t s)
-  | .Rcd t => .Rcd (betar_rcd k t s)
+  | .Rcd tpt tpl => .Rcd (tpt.map (fun t => betar k t s)) tpl
   | .Proj t l => .Proj (betar k t s) l
-where
-  betar_rcd (k : Nat) (t : RcdTerm) (s : Term) : RcdTerm :=
-  match t with
-  | RcdTerm.RcdNil => RcdTerm.RcdNil
-  | RcdTerm.RcdCons l hd tl =>
-    RcdTerm.RcdCons l (betar k hd s) (betar_rcd k tl s)
 
 abbrev subst (t s : Term) : Term := betar 0 t s
 
-def RcdTerm.proj (t : RcdTerm) (l : Label) : Option Term :=
-match t with
-| RcdTerm.RcdNil => none
-| RcdTerm.RcdCons l' hd tl =>
-  if l = l' then some hd else tl.proj l
-
-mutual
 inductive Step : Term → Term → Prop
 | AppL (t t' s : Term) :
   Step t t' →
@@ -236,97 +203,54 @@ inductive Step : Term → Term → Prop
 | IsZero (t t' : Term) :
   Step t t' →
   Step (.IsZero t) (.IsZero t')
-| Rcd (rl : RcdTerm) (rl' : RcdTerm) :
-  RcdStep rl rl' →
-  Step (.Rcd rl) (.Rcd rl')
+| Rcd (tpt : List Term) (tpl : SList Label) (t : Term) (i : Nat) :
+  Step tpt[i]! t →
+  Step (.Rcd tpt tpl) (.Rcd (tpt.set i t) tpl)
 | Proj (t t' : Term) (l : Label) :
   Step t t' →
   Step (.Proj t l) (.Proj t' l)
-| ProjRcd (rl : RcdTerm) (l : Label) (v : Term) :
-  RcdValue rl →
-  rl.proj l = some v →
-  Step (.Proj (.Rcd rl) l) v
-
-inductive RcdStep : RcdTerm → RcdTerm → Prop
-| RcdHere (l : Label) (hd hd' : Term) (tl : RcdTerm) :
-  Step hd hd' →
-  RcdStep (RcdTerm.RcdCons l hd tl) (RcdTerm.RcdCons l hd' tl)
-| RcdThere (l : Label) (hd : Term) (tl tl' : RcdTerm) :
-  Value hd → RcdStep tl tl' →
-  RcdStep (RcdTerm.RcdCons l hd tl) (RcdTerm.RcdCons l hd tl')
-end
+| ProjRcd (tpt : List Term) (tpl : SList Label) (k : Nat) :
+  -- we can do a step under index even if we have duplicates?
+  k < tpl.elems.length →
+  k < tpt.length →
+  Step (.Proj (.Rcd tpt tpl) tpl.elems[k]!) tpt[k]!
 
 lemma beta_typ (tp : type) (S : type) :
-  Typ (Γ₁ ++ Γ) s S → Typ (Γ₁ ++ tp :: Γ) (shift_up_from Γ₁.length s) S := by
-  intro hs
-  cases s <;> try grind [Typ, shift_up_from]
-  · cases hs
-    rename_i htc ht1 ht2
-    have _ := beta_typ tp _ ht1
-    have _ := beta_typ tp _ ht2
-    have _ := beta_typ tp _ htc
-    grind [Typ, shift_up_from]
-  · cases hs
-    rename_i tp' _ ht
-    have _ := beta_typ (Γ₁ := tp' :: Γ₁) tp _ ht
-    grind [Typ, shift_up_from]
-  · sorry
-  · cases hs
-    rename_i ht
-    have _ := beta_typ tp _ ht
-    grind [Typ, shift_up_from]
-  · cases hs
-    rename_i ht
-    have _ := beta_typ tp _ ht
-    grind [Typ, shift_up_from]
-  · sorry
-  · sorry
-  · sorry
+  Γ₂ = Γ₁ ++ Γ → Typ Γ₂ s S → Typ (Γ₁ ++ tp :: Γ) (shift_up_from Γ₁.length s) S := by
+  intro hs hs1
+  induction hs1 generalizing Γ₁ Γ <;> try grind [Typ, shift_up_from]
 
 lemma betar_preservation (t s : Term) (S T : type) (Γ Γ₁ : TCtx) :
-  Typ (Γ₁ ++ Γ) s S → Typ (Γ₁ ++ S :: Γ) t T → Typ (Γ₁ ++ Γ) (betar Γ₁.length t s) T := by
-    intro hs ht
-    unhygienic induction t generalizing Γ Γ₁ s S T
-    all_goals (try grind [Typ, betar])
-    · cases ht
-      rw [betar]
-      split
-      · grind
-      · split
-        · grind [Typ]
-        · grind [Typ]
-    · cases ht
-      rename_i tp2 ih
-      rw [betar]
+  Γ₂ = Γ₁ ++ S :: Γ → Typ (Γ₁ ++ Γ) s S → Typ Γ₂ t T → Typ (Γ₁ ++ Γ) (betar Γ₁.length t s) T := by
+    intro heq hs ht
+    unhygienic induction ht generalizing Γ₁ S s
+    iterate 2 { grind [Typ, betar] }
+    { rw [betar]
+      repeat' split <;> grind [Typ] }
+    { rw [betar]
       apply Typ.TAbs
-      apply t_ih (shift_up s) S tp2 Γ (tp :: Γ₁)
-      · have lm := beta_typ tp (Γ₁ := []) (Γ := Γ₁ ++ Γ) (S := S) (s := s)
-        grind [shift_up]
-      · grind
+      have ih := a_ih (shift_up s) S (tp₁ :: Γ₁) (by grind) (by
+        rw [shift_up]
+        have typ_lm := beta_typ tp₁ S (Γ₁ := []) (Γ := Γ₁ ++ Γ) (by grind) hs
+        grind)
+      grind }
+    all_goals { grind [betar, Typ] }
 
 theorem preservation (t t' : Term) (tp : type) (Γ : TCtx) :
   Step t t' → Typ Γ t tp → Typ Γ t' tp := by
     intro hs ht
-    unhygienic induction hs generalizing Γ tp <;> try grind [Typ]
-    unhygienic cases ht
-    unhygienic cases a_1
-    rename_i tp1
-    have lm := betar_preservation t_1 s tp1 tp Γ []
-    grind
-
-lemma weakening (t : Term) (tp : type) (Γ Γ₁ : TCtx) :
-  Typ Γ t tp → Typ (Γ ++ Γ₁) t tp := by
-    intro ht
-    induction ht <;> grind [Typ]
+    unhygienic induction hs generalizing Γ tp
+    iterate 2 { grind [Typ] }
+    { unhygienic cases ht
+      unhygienic cases a_1
+      rename_i tp1
+      have lm := betar_preservation t_1 s tp1 tp Γ [] (Γ₂ := tp1 :: Γ)
+      grind }
+    iterate 12 { grind [Typ] }
+    grind [Typ]
 
 lemma nat_value_from (ht : Typ Γ t type.nat) (hv : Value t) : NatValue t := by
-  cases ht <;> cases hv
-  · contradiction
-  · contradiction
-  · contradiction
-  · grind
-  · grind
-  · contradiction
+  cases ht <;> cases hv <;> grind
 
 lemma bool_value_from (ht : Typ Γ t type.boolean) (hv : Value t) :
   t = .trueT ∨ t = .falseT := by
@@ -334,7 +258,6 @@ lemma bool_value_from (ht : Typ Γ t type.boolean) (hv : Value t) :
   all_goals (try contradiction)
   · grind
   · grind
-
 theorem progress (t : Term) (td : Typ [] t T) :
   Value t ∨ ∃ t', Step t t' := by
   generalize h : [] = Γ at td
@@ -345,38 +268,43 @@ theorem progress (t : Term) (td : Typ [] t T) :
   · grind [Value]
   · rename_i ht _ ih1 ih2
     cases ih1 h
-    · rename_i hv
+    · rename_i tp₁ tp₂ a hv
+      generalize hp : tp₁.arr tp₂ = tp at ht
       cases ht <;> cases hv
       all_goals (try contradiction)
       cases ih2 h
-      · rename_i t2 _ _ _ _ t _ _
+      · rename_i t2 _ t _ _ _ _
         right
         exists subst t t2
-        grind [Step]
-      · rename_i tp _ _ t _ hs
+        solve_by_elim
+      · rename_i t tp _ _  hs
         have ⟨ t2', _ ⟩ := hs
         right
         exists (t.Abs tp).App t2'
-        grind [Step]
+        solve_by_elim
     · rename_i t2 _ _ _ _ hs
       have ⟨ t1', _ ⟩ := hs
       right
       exists (.App t1' t2)
-      grind [Step]
+      solve_by_elim
   · rename_i ihc iht ihe
     cases ihc h
     · rename_i t1 t2 _ _ _ _ _ _
       right
       cases bool_value_from (by assumption) (by assumption)
       · exists t1
-        grind [Step]
+        rename_i hc
+        rw [hc]
+        solve_by_elim
       · exists t2
-        grind [Step]
+        rename_i hc
+        rw [hc]
+        solve_by_elim
     · rename_i t1 t2 _ _ _ _ _ hs
       have ⟨ ct', _ ⟩ := hs
       right
       exists (.ite ct' t1 t2)
-      grind [Step]
+      solve_by_elim
   · grind [Value, NatValue]
   · rename_i ih
     cases ih h
@@ -387,22 +315,22 @@ theorem progress (t : Term) (td : Typ [] t T) :
       have ⟨ t', _ ⟩ := hs
       right
       exists (.Succ t')
-      grind [Step]
+      solve_by_elim
   · rename_i ih
     cases ih h
     · cases nat_value_from (by assumption) (by assumption)
       · right
         exists .Zero
-        grind [Step]
+        solve_by_elim
       · rename_i t _ _ _
         right
         exists t
-        grind [Step]
+        solve_by_elim
     · rename_i hs
       have ⟨ t', _ ⟩ := hs
       right
       exists (.Pred t')
-      grind [Step]
+      solve_by_elim
   · rename_i ht ih
     cases ih h
     · rename_i hv
@@ -410,13 +338,53 @@ theorem progress (t : Term) (td : Typ [] t T) :
       right
       cases nv
       · exists .trueT
-        grind [Step]
+        solve_by_elim
       · exists .falseT
-        grind [Step]
+        solve_by_elim
     · rename_i hs
       have ⟨ t', _ ⟩ := hs
       right
       exists (.IsZero t')
-      grind [Step]
-
+      solve_by_elim
+  { rename_i tpt _ tpl₁ tpl₂ tps hl1 hl2 hls hd ih
+    by_cases ha : ∀ i < tpt.length, Value tpt[i]!
+    { left
+      apply Value.RcdV
+      solve_by_elim }
+    right
+    simp only [not_forall] at ha
+    rcases ha with ⟨i, ht, htv⟩
+    have ex2 : ∃ j < tpt.length, tpl₁.elems[i]! = tpl₂.elems[j]! := by
+      have : tpt.length = tpl₂.elems.length := by
+        grind [hl2.length_eq]
+      rw [this]
+      rcases SList.Perm.key_correspondence tpl₁ tpl₂ (by grind) ⟨i, by grind⟩ with ⟨j, hj⟩
+      simp at hj
+      grind
+    rcases ex2 with ⟨j, hj⟩
+    cases ih i j (by grind) (by grind [hl2.length_eq]) (by grind) h
+    { grind }
+    rename_i ht
+    rcases ht with ⟨t1, ht1⟩
+    exists Term.Rcd (tpt.set i t1) tpl₁
+    solve_by_elim }
+  right
+  rename_i l _ tpl tps i tp tp₁ htp hk heq ih
+  cases ih h <;> rename_i h1
+  { cases h1
+    iterate 4 grind [Typ, NatValue]
+    rename_i tpt1 tpl1 hv
+    cases tp₁
+    have exi : ∃ j < tpt1.length, tpl1.elems[j]! = tpl.elems[i]! := by
+      rename_i ht1 hsl ht2 ht
+      have := SList.Perm.key_correspondence tpl tpl1 (by grind) ⟨i, by grind⟩
+      grind
+    rcases exi with ⟨j, hj, hq⟩
+    exists tpt1[j]!
+    rw [htp, ←hq]
+    apply Step.ProjRcd tpt1 <;> grind }
+  unhygienic cases h1
+  exists w.Proj l
+  apply Step.Proj
+  apply h_1
 end Subtyping
